hehehe look what I did; we're squashing so I can say what I want

systems/VarDUpgrade.v
@@ -4,7 +4,9 @@ Require Import VarD.
 
 Require Import StringMap.
 
-Module list_to_tree(E : EQUALITY_TYPE) (T : TREE with Definition elt := E.t).
+Module list_to_tree(E : EQUALITY_TYPE) (T : TREE
+                                           with Definition elt := E.t
+                                           with Definition elt_eq := E.eq).
   Module M := ETree(E).
 
   Fixpoint list_to_tree {V} (l : M.t V) : T.t V :=
@@ -12,6 +14,18 @@ Module list_to_tree(E : EQUALITY_TYPE) (T : TREE with Definition elt := E.t).
     | [] => T.empty V
     | (k,v) :: l' => T.set k v (list_to_tree l')
     end.
+
+  Lemma list_to_tree_equiv :
+    forall V (l : M.t V) k,
+      M.get k l = T.get k (list_to_tree l).
+  Proof.
+    induction l; simpl; intros.
+    - now rewrite T.gempty.
+    - destruct a.
+      rewrite T.gsspec.
+      unfold T.elt_eq.
+      break_if; auto.
+  Qed.
 End list_to_tree.
 
 Module LT := list_to_tree EqString LogTimeStringMap.
@@ -25,7 +39,44 @@ Definition simulation (d1 : LinearTimeVarD.data) (d2 : LogTimeVarD.data) : Prop 
 Lemma upgrade_establishes_simulation :
   forall d1,
     simulation d1 (upgrade d1).
-Admitted.
+Proof.
+  unfold simulation.
+  eauto using LT.list_to_tree_equiv.
+Qed.
+
+Lemma set_preserves_simulation :
+  forall d1 d2 k v,
+    simulation d1 d2 ->
+    simulation (VarD.LinearTimeVarD.Map.set k v d1) (VarD.LogTimeVarD.Map.set k v d2).
+Proof.
+  unfold simulation.
+  intros.
+  rewrite LinearTimeStringMap.gsspec, LogTimeStringMap.gsspec.
+  unfold LinearTimeStringMap.elt_eq, LogTimeStringMap.elt_eq.
+  unfold IndexedString.eq, EqString.eq.
+  break_if; auto.
+Qed.
+
+Lemma remove_preserves_simulation :
+  forall d1 d2 k,
+    simulation d1 d2 ->
+    simulation (VarD.LinearTimeVarD.Map.remove k d1) (VarD.LogTimeVarD.Map.remove k d2).
+Proof.
+  unfold simulation.
+  intros.
+  rewrite LinearTimeStringMap.grspec, LogTimeStringMap.grspec.
+  unfold LinearTimeStringMap.elt_eq, LogTimeStringMap.elt_eq.
+  unfold IndexedString.eq, EqString.eq.
+  break_if; auto.
+Qed.
+
+Lemma simulation_get :
+  forall d1 d2 k,
+    simulation d1 d2 ->
+    VarD.LinearTimeVarD.Map.get k d1 = VarD.LogTimeVarD.Map.get k d2.
+Proof.
+  auto.
+Qed.
 
 Theorem handlers_preserve_simulation :
   forall d1 d2 d1' i o,
@@ -34,7 +85,48 @@ Theorem handlers_preserve_simulation :
     exists d2',
       simulation d1' d2' /\
       LogTimeVarD.VarDHandler i d2 = (o, d2').
-Admitted.
+Proof.
+  destruct i eqn:?; simpl; intros;
+    unfold StateMachineHandlerMonad.bind in *; repeat break_let; repeat find_inversion.
+  - unfold LinearTimeVarD.resp, LogTimeVarD.resp in *.
+    unfold LinearTimeVarD.setk, LogTimeVarD.setk in *.
+    unfold LinearTimeVarD.getk, LogTimeVarD.getk in *.
+    StateMachineHandlerMonad.monad_unfold.
+    repeat find_inversion.
+    eexists. intuition eauto using f_equal2.
+    auto using set_preserves_simulation.
+  - unfold LinearTimeVarD.resp, LogTimeVarD.resp in *.
+    unfold LinearTimeVarD.setk, LogTimeVarD.setk in *.
+    unfold LinearTimeVarD.getk, LogTimeVarD.getk in *.
+    StateMachineHandlerMonad.monad_unfold.
+    repeat find_inversion.
+    eauto using f_equal2.
+  - unfold LinearTimeVarD.resp, LogTimeVarD.resp in *.
+    unfold LinearTimeVarD.delk, LogTimeVarD.delk in *.
+    unfold LinearTimeVarD.getk, LogTimeVarD.getk in *.
+    StateMachineHandlerMonad.monad_unfold.
+    repeat find_inversion.
+    eexists. intuition eauto using f_equal2.
+    auto using remove_preserves_simulation.
+  - unfold LinearTimeVarD.resp, LogTimeVarD.resp in *.
+    unfold LinearTimeVarD.setk, LogTimeVarD.setk in *.
+    unfold LinearTimeVarD.getk, LogTimeVarD.getk in *.
+    StateMachineHandlerMonad.monad_unfold.
+    repeat find_inversion.
+    erewrite simulation_get in * by eauto.
+    repeat break_if; try congruence; repeat find_inversion;
+    eexists; intuition eauto using f_equal2;
+    eauto using set_preserves_simulation.
+  - unfold LinearTimeVarD.resp, LogTimeVarD.resp in *.
+    unfold LinearTimeVarD.delk, LogTimeVarD.delk in *.
+    unfold LinearTimeVarD.getk, LogTimeVarD.getk in *.
+    StateMachineHandlerMonad.monad_unfold.
+    repeat find_inversion.
+    erewrite simulation_get in * by eauto.
+    repeat break_if; try congruence; repeat find_inversion;
+    eexists; intuition eauto using f_equal2;
+    eauto using remove_preserves_simulation.
+Qed.
 
 Instance vard_upgrade_params : StateMachineUpgradeParams :=
  {
